\documentclass{article}
\usepackage{amssymb}
\usepackage{amsmath}
\usepackage{centernot}

\begin{document}

\title{M361K\: Homework 1}
\author{Joshua Dong}
\date{\today}
\maketitle

\subsection{1.2.1}
Prove that $\frac{1}{1 \cdot 2} + \frac{1}{2 \cdot 3} + \ldots +
\frac{1}{n (n+1)} = \frac{n}{n+1} \forall \; n \in \mathbb{N}$
\\Let $P(x)$ be the statement: $\frac{1}{1 \cdot 2} + \frac{1}{2 \cdot 3} +
\ldots + \frac{1}{x (x+1)} = \frac{x}{x+1}$.
\\$\frac{1}{1 \cdot 2} = \frac{1}{1+1}$.
\\$\therefore P(0)$ holds.
\\$\therefore P(n)$ for some $n \in \mathbb{N}$.
\\$\frac{1}{1 \cdot 2} + \frac{1}{2 \cdot 3} + \ldots +
\frac{1}{n (n+1)} + \frac{1}{(n+1)(n+2)} =
\\\frac{n}{n+1} + \frac{1}{(n+1)(n+2)} =
\frac{n(n+2)}{(n+1)(n+2)} + \frac{1}{(n+1)(n+2)} =
\frac{n(n+2)+1}{(n+1)(n+2)} = \frac{n^2+2n+1}{(n+1)(n+2)} =
\frac{n+1}{n+2}$.
\\$\therefore P(n) \rightarrow P(n+1)$.
\\$\therefore P(n) \; \forall \; n \in \mathbb{N}$.

\subsection{1.2.4}
Prove that $1^3 + 2^3 + \ldots + (2n-1)^2 =
\frac{4n^3-n}{3} \; \forall \; n \in \mathbb{N}$
\\Let $P(n)$ be the statement: $1^3 + 2^3 + \ldots + (2n-1)^2 =
\frac{4n^3-n}{3}$.
\\$1^3 = \frac{4 \cdot 1^3-1}{3}$
\\$\therefore P(0)$ holds.
\\$\therefore P(n)$ for some $n \in \mathbb{N}$.
\\$1^3 + 2^3 + \ldots + (2n-1)^2 + (2n+1)^2 =
\frac{4n^3-n}{3} + (2n+1)^2 =
\\\frac{4n^3-n}{3} + \frac{3(4n^2+4n+1)}{3} =
\frac{4n^3-n+12n^2+12n+3}{3} = \frac{4n^3+12n^2+11n+3}{3} = 
\frac{4(n^3+3n^2+3n+1)-(n+1)}{3} = 
\frac{4(n+1)^3-(n+1)}{3}$.
\\$\therefore P(n) \rightarrow P(n+1)$.
\\$\therefore P(n) \; \forall \; n \in \mathbb{N}$.

\subsection{1.2.8}
Prove that $1^3 + 2^3 + \ldots + (2n-1)^2 =
\frac{4n^3-n}{3} \; \forall \; n \in \mathbb{N}$
\\Let $P(n)$ be the statement: $1^3 + 2^3 + \ldots + (2n-1)^2 =
\frac{4n^3-n}{3}$.
\\$1^3 = \frac{4 \cdot 1^3-1}{3}$
\\$\therefore P(0)$ holds.
\\$\therefore P(n)$ for some $n \in \mathbb{N}$.
\\$1^3 + 2^3 + \ldots + (2n-1)^2 =
\frac{4n^3-n}{3}$.
\\$\therefore P(n) \rightarrow P(n+1)$.
\\$\therefore P(n) \; \forall \; n \in \mathbb{N}$.

\subsection{1.2.13}

\subsection{1.2.18}

\subsection{1.2.20}

\end{document}
